{
 "cells": [
  {
   "cell_type": "markdown",
   "metadata": {},
   "source": [
    "The first way (least square)\n",
    "\n",
    "$$\n",
    "{w_{RR}} = \\arg \\mathop {\\min }\\limits_w {\\left\\| {y - Xw} \\right\\|^2} + \\lambda g\\left( w \\right)\n",
    "$$\n",
    "\n",
    "$${w_{RR}} = \\arg \\mathop {\\min }\\limits_w {\\left\\| {y - Xw} \\right\\|^2} + \\lambda {\\left\\| w \\right\\|^2}$$\n",
    "\n",
    "We have:\n",
    "\n",
    "$L = {\\left\\| {y - Xw} \\right\\|^2} + \\lambda {\\left\\| w \\right\\|^2}$\n",
    "\n",
    "$ {\\nabla _w}L = {\\nabla _w}\\left( {{{\\left\\| {y - Xw} \\right\\|}^2} + \\lambda {{\\left\\| w \\right\\|}^2}} \\right)$\n",
    "\n",
    "$ {\\nabla _w}L = {\\nabla _w}\\left( {{{\\left( {y - Xw} \\right)}^T}\\left( {y - Xw} \\right) + \\lambda {w^T}w} \\right)$\n",
    "\n",
    "\n",
    "$ {\\nabla _w}L = {\\nabla _w}\\left( {{y^T}y - {y^T}Xw - {w^T}{X^T}y + {w^T}{X^T}Xw + \\lambda {w^T}w} \\right)$\n",
    "\n",
    "${\\nabla _w}L = {\\nabla _w}\\left( { - {w^T}{X^T}y - {w^T}{X^T}y + {w^T}{X^T}Xw + \\lambda {w^T}w} \\right)$\n",
    "\n",
    "$\\Rightarrow  - 2{X^T}y + 2{X^T}Xw + 2\\lambda w = 0$\n",
    "\n",
    "$\\Leftrightarrow \\left( {2{X^T}X + 2\\lambda I} \\right)w = 2{X^T}y$\n",
    "\n",
    "$\\Leftrightarrow w = {\\left( {{X^T}X + \\lambda I} \\right)^{ - 1}}{X^T}y$\n",
    "\n"
   ]
  },
  {
   "cell_type": "markdown",
   "metadata": {},
   "source": [
    "The second way: Maximum Posterior\n",
    "\n",
    "\n",
    "We have:\n",
    "\n",
    "$\n",
    "{w_{MAP}} = \\arg \\mathop {\\max }\\limits_w \\ln p\\left( {w|y,X} \\right)\n",
    "$\n",
    "\n",
    "$\n",
    " {w_{MAP}} = \\arg \\mathop {\\max }\\limits_w \\ln \\frac{{p\\left( {y|w,X} \\right)p\\left( w \\right)}}{{p\\left( {y|X} \\right)}}\n",
    "$\n",
    "\n",
    "$\n",
    " {w_{MAP}} = \\arg \\mathop {\\max }\\limits_w \\left( {\\ln p\\left( {y|w,X} \\right) + \\ln p\\left( w \\right) - \\ln p\\left( {y|X} \\right)} \\right)\n",
    "$\n",
    "\n",
    "Because ${\\ln p\\left( {y|X} \\right)}$ doesn't involve $w$, so we can maximize $\\ln p\\left( {y|w,X} \\right) + \\ln p\\left( w \\right)$:\n",
    "\n",
    "$\n",
    " {w_{MAP}} = \\arg \\mathop {\\max }\\limits_w \\left( {\\ln p\\left( {y|w,X} \\right) + \\ln p\\left( w \\right)} \\right)\n",
    "$\n",
    "\n",
    "$\n",
    " {w_{MAP}} = \\arg \\mathop {\\max }\\limits_w \\left( {\\ln \\frac{1}{{\\sigma \\sqrt {2\\pi } }}\\exp \\left( { - \\frac{{{{\\left( {y - Xw} \\right)}^T}\\left( {y - Xw} \\right)}}{{2{\\sigma ^2}}}} \\right) + \\ln \\left( {{{\\left( {\\frac{\\lambda }{{2\\pi }}} \\right)}^{\\frac{d}{2}}}\\exp \\left( { - \\frac{\\lambda }{2}{w^T}w} \\right)} \\right)} \\right)\n",
    "$\n",
    "\n",
    "$\n",
    " {w_{MAP}} = \\arg \\mathop {\\max }\\limits_w \\left( {\\ln \\frac{1}{{\\sigma \\sqrt {2\\pi } }} + \\ln \\exp \\left( { - \\frac{{{{\\left( {y - Xw} \\right)}^T}\\left( {y - Xw} \\right)}}{{2{\\sigma ^2}}}} \\right) + \\ln {{\\left( {\\frac{\\lambda }{{2\\pi }}} \\right)}^{\\frac{d}{2}}} + \\ln \\exp \\left( { - \\frac{\\lambda }{2}{w^T}w} \\right)} \\right)\n",
    "$\n",
    "\n",
    "$\n",
    " {w_{MAP}} = \\arg \\mathop {\\max }\\limits_w \\left( { - \\frac{1}{{2{\\sigma ^2}}}{{\\left( {y - Xw} \\right)}^T}\\left( {y - Xw} \\right) - \\frac{\\lambda }{2}{w^T}w + \\ln \\frac{1}{{\\sigma \\sqrt {2\\pi } }} + \\ln {{\\left( {\\frac{\\lambda }{{2\\pi }}} \\right)}^{\\frac{d}{2}}}} \\right)\n",
    "$\n",
    "\n",
    "Call:\n",
    "\n",
    "$\n",
    " L =  - \\frac{1}{{2{\\sigma ^2}}}{\\left( {y - Xw} \\right)^T}\\left( {y - Xw} \\right) - \\frac{\\lambda }{2}{w^T}w + \\ln \\frac{1}{{\\sigma \\sqrt {2\\pi } }} + \\ln {\\left( {\\frac{\\lambda }{{2\\pi }}} \\right)^{\\frac{d}{2}}}\n",
    "$\n",
    "\n",
    "$\n",
    " \\Rightarrow {\\nabla _w}L = {\\nabla _w}\\left( { - \\frac{1}{{2{\\sigma ^2}}}{{\\left( {y - Xw} \\right)}^T}\\left( {y - Xw} \\right) - \\frac{\\lambda }{2}{w^T}w + \\ln \\frac{1}{{\\sigma \\sqrt {2\\pi } }} + \\ln {{\\left( {\\frac{\\lambda }{{2\\pi }}} \\right)}^{\\frac{d}{2}}}} \\right)\n",
    "$\n",
    "\n",
    "$\n",
    "{\\nabla _w}L = {\\nabla _w}\\left( { - \\frac{1}{{2{\\sigma ^2}}}{{\\left( {y - Xw} \\right)}^T}\\left( {y - Xw} \\right)} \\right) + {\\nabla _w}\\left( { - \\frac{\\lambda }{2}{w^T}w} \\right) + \\underbrace {{\\nabla _w}\\left( {\\ln \\frac{1}{{\\sigma \\sqrt {2\\pi } }} + \\ln {{\\left( {\\frac{\\lambda }{{2\\pi }}} \\right)}^{\\frac{d}{2}}}} \\right)}_0\n",
    "$\n",
    "\n",
    "$\n",
    "{\\nabla _w}L = {\\nabla _w}\\left( { - \\frac{1}{{2{\\sigma ^2}}}\\left( {y{y^T} - {y^T}Xw - {w^T}{X^T}y + {w^T}{X^T}Xw} \\right)} \\right) + {\\nabla _w}\\left( { - \\frac{\\lambda }{2}{w^T}w} \\right)\n",
    "$\n",
    "\n",
    "$\n",
    "\\Rightarrow  {\\nabla _w}L = \\frac{1}{{{\\sigma ^2}}}{X^T}y - \\frac{1}{{{\\sigma ^2}}}{X^T}Xw - \\lambda w = 0\n",
    "$\n",
    "\n",
    "$\n",
    "\\Leftrightarrow  \\frac{1}{{{\\sigma ^2}}}{X^T}Xw + \\lambda w = \\frac{1}{{{\\sigma ^2}}}{X^T}y\n",
    "$\n",
    "\n",
    "$\n",
    "\\Leftrightarrow {X^T}Xw + {\\sigma ^2}\\lambda w = {X^T}y\n",
    "$\n",
    "\n",
    "$\n",
    "\\Leftrightarrow \\left( {{X^T}X + {\\sigma ^2}\\lambda } \\right)w = {X^T}y\n",
    "$\n",
    "\n",
    "$\n",
    "\\Leftrightarrow \\left( {{X^T}X + {\\sigma ^2}\\lambda } \\right)w = {X^T}y\n",
    "$\n",
    "\n",
    "$\n",
    "\\Leftrightarrow w = {\\left( {{X^T}X + {\\sigma ^2}\\lambda } \\right)^{ - 1}}{X^T}y\n",
    "$"
   ]
  }
 ],
 "metadata": {
  "kernelspec": {
   "display_name": "Python 3",
   "language": "python",
   "name": "python3"
  },
  "language_info": {
   "codemirror_mode": {
    "name": "ipython",
    "version": 3
   },
   "file_extension": ".py",
   "mimetype": "text/x-python",
   "name": "python",
   "nbconvert_exporter": "python",
   "pygments_lexer": "ipython3",
   "version": "3.8.2"
  }
 },
 "nbformat": 4,
 "nbformat_minor": 4
}
